theories/Props/Prop/Rewriting.v
@@ -1,0 +1,1703 @@
+(* A file containing rewriting theory, especially for rewriting in
+  autonomous and frobenius categories *)
+
+From TensorRocq Require Import CospanHyperGraph.Definitions
+  Isomorphism.IsoAux Isomorphism.Testing CospanHyperGraph.Matching
+  Props.Prop.Props
+  Props.Prop.PropsGraphs.
+  (* Props.Prop.PropGraphTerm. *)
+
+
+
+(* FIXME: Move?!?!?!? *)
+
+Import StackComposeCorrect.
+
+#[export] Instance compose_graphs_alt_cohg_vert_eq {T}
+  {n m o} : Proper (cohg_vert_eq ==> cohg_vert_eq ==> cohg_vert_eq)
+    (@compose_graphs_alt T n m o).
+Proof.
+  intros cohg1 cohg1' Hcohg1 cohg2 cohg2' Hcohg2.
+  unfold compose_graphs_alt.
+  now do 2 f_equiv.
+Qed.
+
+#[export] Instance compose_graphs_alt_struct_isomorphic `{Equiv T, Equivalence T equiv}
+  {n m o} : Proper (struct_isomorphic ==> struct_isomorphic ==> struct_isomorphic)
+    (@compose_graphs_alt T n m o).
+Proof.
+  intros cohg1 cohg1' Hcohg1 cohg2 cohg2' Hcohg2.
+  unfold compose_graphs_alt.
+  apply add_top_loops_struct_isomorphic.
+  now apply swapped_stack_graphs_struct_isomorphic.
+Qed.
+
+Import Facts.
+
+Lemma proper_cohg_syntactic_eq_of_struct_iso_eq_binary `{Equiv T1, Equivalence T1 equiv,
+  Equiv T2, Equivalence T2 equiv, Equiv T3, Equivalence T3 equiv} {n1 m1 n2 m2 n3 m3}
+  (f : CospanHyperGraph T1 n1 m1 -> CospanHyperGraph T2 n2 m2 ->
+    CospanHyperGraph T3 n3 m3) :
+  Proper (struct_isomorphic ==> struct_isomorphic ==> struct_isomorphic) f ->
+  Proper (cohg_eq ==> cohg_eq ==> cohg_eq) f ->
+  Proper (cohg_syntactic_eq ==> cohg_syntactic_eq ==> cohg_syntactic_eq) f.
+Proof.
+  intros Hfiso Hfcohg.
+  intros cohg1 cohg1' Hcohg1 cohg2 cohg2' Hcohg2.
+  induction Hcohg1 as [cohg1 cohg1' fv1 fe1 Hfv1 Hfe1 Hverteq1].
+  rewrite <- (subrel'' struct_isomorphic (norm_verts_vert_eq cohg1)).
+  rewrite (Hverteq1).
+  rewrite (subrel'' struct_isomorphic (norm_verts_vert_eq _)).
+  rewrite <- (subrel'' struct_isomorphic (iso_relabel_reindex _ _ _)) by done.
+  induction Hcohg2 as [cohg2 cohg2' fv2 fe2 Hfv2 Hfe2 Hverteq2].
+  rewrite <- (subrel'' struct_isomorphic (norm_verts_vert_eq cohg2)).
+  rewrite (Hverteq2).
+  rewrite (subrel'' struct_isomorphic (norm_verts_vert_eq _)).
+  rewrite <- (subrel'' struct_isomorphic (iso_relabel_reindex _ _ _)) by done.
+  done.
+Qed.
+
+#[export] Instance compose_graphs_alt_cohg_syntactic_eq `{Equiv T, Equivalence T equiv}
+  {n m o} : Proper (cohg_syntactic_eq ==> cohg_syntactic_eq ==> cohg_syntactic_eq)
+    (@compose_graphs_alt T n m o).
+Proof.
+  apply proper_cohg_syntactic_eq_of_struct_iso_eq_binary; apply _.
+Qed.
+
+#[export] Instance compose_graphs_cohg_vert_eq {T}
+  {n m o} : Proper (cohg_vert_eq ==> cohg_vert_eq ==> cohg_vert_eq)
+    (@compose_graphs T n m o).
+Proof.
+  intros cohg1 cohg1' Hcohg1 cohg2 cohg2' Hcohg2.
+  do 2 rewrite <- compose_graphs_alt_correct.
+  now do 2 f_equiv.
+Qed.
+
+#[export] Instance compose_graphs_struct_isomorphic `{Equiv T, Equivalence T equiv}
+  {n m o} : Proper (struct_isomorphic ==> struct_isomorphic ==> struct_isomorphic)
+    (@compose_graphs T n m o).
+Proof.
+  intros cohg1 cohg1' Hcohg1 cohg2 cohg2' Hcohg2.
+  do 2 rewrite <- compose_graphs_alt_correct.
+  now apply compose_graphs_alt_struct_isomorphic.
+Qed.
+
+#[export] Instance compose_graphs_cohg_syntactic_eq `{Equiv T, Equivalence T equiv}
+  {n m o} : Proper (cohg_syntactic_eq ==> cohg_syntactic_eq ==> cohg_syntactic_eq)
+    (@compose_graphs T n m o).
+Proof.
+  intros cohg1 cohg1' Hcohg1 cohg2 cohg2' Hcohg2.
+  rewrite <- 2 compose_graphs_alt_correct.
+  now apply compose_graphs_alt_cohg_syntactic_eq.
+Qed.
+
+#[export] Instance stack_graphs_cohg_syntactic_eq `{Equiv T, Equivalence T equiv}
+  {n m o p} : Proper (cohg_syntactic_eq ==> cohg_syntactic_eq ==> cohg_syntactic_eq)
+    (@stack_graphs T n m o p).
+Proof.
+  apply proper_cohg_syntactic_eq_of_iso_vert_eq_binary; apply _.
+Qed.
+
+
+
+
+From TensorRocq Require Import ProQuote.
+From TensorRocq Require Import CospanHyperGraph.Hom.
+
+(* FIXME: Move to Definitions *)
+Lemma cohg_eq_ind `{Equiv T} {n m} (P : CospanHyperGraph T n m -> CospanHyperGraph T n m -> Prop)
+  (HP : forall ins outs verts he he', map_equiv he he' ->
+    P (mk_cohg (mk_hg he verts) ins outs) (mk_cohg (mk_hg he' verts) ins outs)) :
+  forall cohg cohg', cohg ≡ₕ cohg' -> P cohg cohg'.
+Proof.
+  intros [[he verts] ins outs] [[he' verts'] ins' outs'] ([= <-] & [= <-] & [Hhe [= <-]]).
+  apply HP, Hhe.
+Qed.
+
+Lemma cohg_eq_ind' `{Equiv T} {n m} (P : CospanHyperGraph T n m -> CospanHyperGraph T n m -> Prop)
+  (HP : forall ins outs hg hg', hg ≡ hg' ->
+    P (mk_cohg hg ins outs) (mk_cohg hg' ins outs)) :
+  forall cohg cohg', cohg ≡ₕ cohg' -> P cohg cohg'.
+Proof.
+  intros [hg ins outs] [hg' ins' outs'] ([= <-] & [= <-] & Hhg).
+  apply HP, Hhg.
+Qed.
+
+#[export] Instance compose_graphs_aux_cohg_eq `{Equiv T} {n m o} :
+  Proper (cohg_eq ==> cohg_eq ==> cohg_eq) (@compose_graphs_aux T n m o).
+Proof.
+  refine (cohg_eq_ind _ _).
+  intros ins1 outs1 verts1 he1 he1' Hhe1.
+  refine (cohg_eq_ind _ _).
+  intros ins2 outs2 verts2 he2 he2' Hhe2.
+  unfold compose_graphs_aux.
+  cbn.
+  f_equiv.
+  split_and!; [done..|].
+  cbn.
+  split; cbn.
+  - now apply fin_maps.union_proper.
+  - do 3 f_equal;
+    eapply vertices_hg_equiv; split; done.
+Qed.
+
+
+#[export] Instance compose_graphs_cohg_eq `{Equiv T} {n m o} :
+  Proper (cohg_eq ==> cohg_eq ==> cohg_eq) (@compose_graphs T n m o).
+Proof.
+  intros cohg1 cohg1' Hcohg1 cohg2 cohg2' Hcohg2.
+  rewrite 2 compose_graphs_to_compose_graphs_aux.
+  now apply compose_graphs_aux_cohg_eq; do 2 f_equiv.
+Qed.
+
+
+(* FIXME: Move *)
+Lemma PRO_graph_semantics_equiv_cohg_eq `{StructGraphable Struct T,
+  EqStruct : forall n m, Equiv (Struct n m),
+  EqT : Equiv T, EquivT : Equivalence T equiv}
+  {GraphSProper : forall n m, Proper ((≡@{Struct n m}) ==> cohg_eq) graph_of_struct}
+  {n m} :
+  Proper ((≡@{PRO Struct T n m}) ==> cohg_eq) PRO_graph_semantics.
+Proof.
+  intros p p' Hp.
+  induction Hp.
+  - done.
+  - cbn.
+    now f_equiv.
+  - cbn.
+    now apply graph_of_tensor_cohg_eq.
+  - cbn.
+    now apply compose_graphs_cohg_eq.
+  - cbn.
+    now apply stack_graphs_cohg_eq.
+Qed.
+
+Lemma PRO_graph_semantics_equiv_cohg_syntactic_eq `{StructGraphable Struct T,
+  EqStruct : forall n m, Equiv (Struct n m),
+  EqT : Equiv T, EquivT : Equivalence T equiv}
+  {GraphSProper : forall n m, Proper ((≡@{Struct n m}) ==> cohg_syntactic_eq) graph_of_struct}
+  {n m} :
+  Proper ((≡@{PRO Struct T n m}) ==> cohg_syntactic_eq) PRO_graph_semantics.
+Proof.
+  intros p p' Hp.
+  induction Hp.
+  - done.
+  - cbn.
+    now f_equiv.
+  - cbn.
+    now apply (subrel' cohg_eq), graph_of_tensor_cohg_eq.
+  - cbn.
+    now apply compose_graphs_cohg_syntactic_eq.
+  - cbn.
+    now apply stack_graphs_cohg_syntactic_eq.
+Qed.
+
+Lemma PRO_graph_semantics_map_full_gen `{StructGraphable Struct T,
+  EqStruct : forall n m, Equiv (Struct n m),
+  EqT : Equiv T, EquivT : Equivalence T equiv}
+  `{StructGraphable Struct' T',
+  EqStruct' : forall n m, Equiv (Struct' n m),
+  EqT' : Equiv T', EquivT' : Equivalence T' equiv}
+  (R : forall n m, relation (CospanHyperGraph T' n m))
+  (HR : forall n m, Equivalence (R n m))
+  (HRcomp : forall n m o, Proper (R n m ==> R m o ==> R n o) (@compose_graphs T' n m o))
+  (HRstack : forall n m o p, Proper (R n m ==> R o p ==> R _ _) (@stack_graphs T' n m o p))
+  (fs : forall n m, Struct n m -> Struct' n m)
+  (ft : T -> T')
+  (Hfs : forall n m s, R n m (graph_apply_hom ft (graph_of_struct s)) (graph_of_struct (fs n m s)))
+  {n m} (p : PRO Struct T n m) :
+  R n m (PRO_graph_semantics (map_PRO fs ft p))
+    (graph_apply_hom ft (PRO_graph_semantics p)).
+Proof.
+  induction p.
+  - done.
+  - cbn.
+    rewrite graph_apply_hom_compose_graphs.
+    f_equiv; done.
+  - cbn.
+    rewrite graph_apply_hom_stack_graphs.
+    f_equiv; done.
+  - cbn.
+    done.
+  - cbn.
+    done.
+Qed.
+
+
+Lemma PRO_graph_semantics_map_cohg_syntactic_eq `{StructGraphable Struct T,
+  EqStruct : forall n m, Equiv (Struct n m),
+  EqT : Equiv T, EquivT : Equivalence T equiv}
+  `{StructGraphable Struct' T',
+  EqStruct' : forall n m, Equiv (Struct' n m),
+  EqT' : Equiv T', EquivT' : Equivalence T' equiv}
+  (fs : forall n m, Struct n m -> Struct' n m)
+  (ft : T -> T')
+  (Hfs : forall n m s, graph_apply_hom ft (graph_of_struct s) ≡ₛ graph_of_struct (fs n m s))
+  {n m} (p : PRO Struct T n m) :
+  PRO_graph_semantics (map_PRO fs ft p) ≡ₛ
+    graph_apply_hom ft (PRO_graph_semantics p).
+Proof.
+  apply PRO_graph_semantics_map_full_gen.
+  - apply _.
+  - intros; apply compose_graphs_cohg_syntactic_eq.
+  - intros; apply stack_graphs_cohg_syntactic_eq.
+  - done.
+Qed.
+
+(* FIXME: Move to PropsGraphs *)
+Class FreeStructGraphable (Struct : Mor nat)
+  `{StructG : forall T, StructGraphable Struct T} :=
+  graph_of_struct_free T {n m} (s : Struct n m) :
+    graph_of_struct (T:=T) s = graph_apply_hom (Empty_set_rect _) (graph_of_struct s).
+
+Lemma free_struct_graphable_empty `{FreeGraphS : FreeStructGraphable Struct}
+  T {n m} (s : Struct n m) : hyperedges (graph_of_struct (T:=T) s) = ∅.
+Proof.
+  rewrite graph_of_struct_free.
+  cbn.
+  apply fmap_empty_iff.
+  apply map_empty.
+  intros i.
+  destruct (_ !! i) as [[[]]|]; done.
+Qed.
+
+Lemma graph_apply_hom_free_graph_of_struct `{FreeGraphS : FreeStructGraphable Struct}
+  {T T'} (f : T -> T') {n m} (s : Struct n m) :
+    graph_apply_hom f (graph_of_struct s) = graph_of_struct s.
+Proof.
+  rewrite (graph_of_struct_free T), (graph_of_struct_free T').
+  rewrite graph_apply_hom_compose.
+  apply graph_apply_hom_ext; done.
+Qed.
+
+#[export] Instance morunion_free_graphable
+  `{FreeGraphS : FreeStructGraphable Struct,
+    FreeGraphS' : FreeStructGraphable Struct'} : FreeStructGraphable (MorUnion Struct Struct').
+Proof.
+  intros T n m [s|s]; cbn; apply graph_of_struct_free.
+Qed.
+
+#[export] Instance monoidal_free_graphable : FreeStructGraphable Monoidal.
+Proof.
+  intros T n m []; done.
+Qed.
+
+#[export] Instance symmetry_free_graphable : FreeStructGraphable Symmetry.
+Proof.
+  intros T n m []; done.
+Qed.
+
+#[export] Instance autonomy_free_graphable : FreeStructGraphable Autonomy.
+Proof.
+  intros T n m []; done.
+Qed.
+
+#[export] Instance frobenial_free_graphable : FreeStructGraphable Frobenial.
+Proof.
+  intros T n m []; done.
+Qed.
+
+
+Class SubStructGraphable (Struct Struct' : Mor nat) (T : Type) `{Equiv T}
+  `{!SubStruct Struct Struct'}
+  `{StructGraphable Struct T, StructGraphable Struct' T} :=
+  graph_of_struct_includeStruct : forall {n m} (s : Struct n m),
+  graph_of_struct (includeStruct s :> Struct' n m) ≡ₛ
+  graph_of_struct s.
+
+#[export] Instance substruct_graphable_refl `{Equiv T, Equivalence T equiv}
+  `{StructGraphable Struct T} :
+  SubStructGraphable Struct Struct T.
+Proof.
+  intros n m s.
+  done.
+Qed.
+
+#[export] Instance substruct_graphable_monoidal_symmetricg
+  `{Equiv T, Equivalence T equiv} :
+  SubStructGraphable Monoidal SymmetricG T.
+Proof.
+  intros n m s.
+  done.
+Qed.
+
+#[export] Instance substruct_graphable_monoidal_autonomous
+  `{Equiv T, Equivalence T equiv} :
+  SubStructGraphable Monoidal Autonomous T.
+Proof.
+  intros n m s.
+  done.
+Qed.
+
+#[export] Instance substruct_graphable_monoidal_frobenius
+  `{Equiv T, Equivalence T equiv} :
+  SubStructGraphable Monoidal Frobenius T.
+Proof.
+  intros n m s.
+  done.
+Qed.
+
+#[export] Instance substruct_graphable_symmetry_symmetricg
+  `{Equiv T, Equivalence T equiv} :
+  SubStructGraphable Symmetry SymmetricG T.
+Proof.
+  intros n m s.
+  done.
+Qed.
+
+#[export] Instance substruct_graphable_symmetry_autonomous
+  `{Equiv T, Equivalence T equiv} :
+  SubStructGraphable Symmetry Autonomous T.
+Proof.
+  intros n m s.
+  done.
+Qed.
+
+#[export] Instance substruct_graphable_symmetry_frobenius
+  `{Equiv T, Equivalence T equiv} :
+  SubStructGraphable Symmetry Frobenius T.
+Proof.
+  intros n m s.
+  done.
+Qed.
+
+#[export] Instance substruct_graphable_autonomy_autonomous
+  `{Equiv T, Equivalence T equiv} :
+  SubStructGraphable Autonomy Autonomous T.
+Proof.
+  intros n m s.
+  done.
+Qed.
+
+#[export] Instance substruct_graphable_autonomy_frobenius
+  `{Equiv T, Equivalence T equiv} :
+  SubStructGraphable Autonomy Frobenius T.
+Proof.
+  intros n m s.
+  done.
+Qed.
+
+#[export] Instance substruct_graphable_frobenial_frobenius
+  `{Equiv T, Equivalence T equiv} :
+  SubStructGraphable Frobenial Frobenius T.
+Proof.
+  intros n m s.
+  done.
+Qed.
+
+#[export] Instance substruct_graphable_symmetricg_autonomous
+  `{Equiv T, Equivalence T equiv} :
+  SubStructGraphable SymmetricG Autonomous T.
+Proof.
+  intros n m s.
+  done.
+Qed.
+
+#[export] Instance substruct_graphable_autonomous_frobenius
+  `{Equiv T, Equivalence T equiv} :
+  SubStructGraphable Autonomous Frobenius T.
+Proof.
+  intros n m s.
+  done.
+Qed.
+
+
+
+
+Lemma PRO_graph_semantics_denote `{FreeStructGraphable Struct,
+  EqStruct : forall n m, Equiv (Struct n m),
+  EqT : Equiv T, EquivT : Equivalence T equiv,
+  EqT' : Equiv T', EquivT' : Equivalence T' equiv}
+  (ft : T -> T')
+  {n m} (p : PRO Struct T n m) :
+  PRO_graph_semantics (PRO_denote ft p) =
+    graph_apply_hom ft (PRO_graph_semantics p).
+Proof.
+  unfold PRO_denote.
+  apply PRO_graph_semantics_map_full_gen; [cbn; apply _..|].
+  intros ? ? s.
+  apply graph_apply_hom_free_graph_of_struct.
+Qed.
+
+Lemma PRO_quote_correct_graph_semantics `{FreeStructGraphable Struct,
+  EqStruct : forall n m, Equiv (Struct n m),
+  EqT : Equiv T, EquivT : Equivalence T equiv,
+  EqT' : Equiv T', EquivT' : Equivalence T' equiv}
+  {StructGProp : forall T (EqT : Equiv T) n m,
+    Proper ((≡@{Struct n m}) ==> cohg_syntactic_eq) (graph_of_struct (T:=T))}
+  (ft : T -> T') {Hft : Proper (equiv ==> equiv) ft}
+  {n m} (qp : PRO Struct T n m) p : PRO_quote ft qp p ->
+  PRO_graph_semantics p ≡ₛ graph_apply_hom ft (PRO_graph_semantics qp).
+Proof.
+  unfold PRO_quote.
+  intros Hp.
+  erewrite <- PRO_graph_semantics_equiv_cohg_syntactic_eq by apply Hp.
+  now rewrite PRO_graph_semantics_denote.
+Qed.
+
+
+
+
+
+
+
+
+
+
+
+
+
+
+
+
+
+Local Existing Instance Countable_Equiv.
+
+
+Record LawfulPRORewritingRelation {Struct T} {StructG : StructGraphable Struct T}
+  `{EqT : Equiv T, EquivT : Equivalence T equiv}
+   := mk_LawfulPRORewritingRelation {
+  pro_rewriting_relation n m : relation (PRO Struct T n m);
+  pro_rewriting_domain {n m} : PRO Struct T n m -> Prop;
+  pro_rewriting_domain_dec {n m} (p : PRO Struct T n m) :: Decision (pro_rewriting_domain p);
+  pro_rewriting_domain_id n : pro_rewriting_domain (Pid n);
+  pro_rewriting_domain_struct {n m} (s : Struct n m) : pro_rewriting_domain ([str s]);
+  pro_rewriting_domain_compose {n m o} (p : PRO Struct T n m) (q : PRO Struct T m o) :
+    pro_rewriting_domain p -> pro_rewriting_domain q -> pro_rewriting_domain (p ;; q);
+  pro_rewriting_domain_stack {n m n' m'} (p : PRO Struct T n m) (q : PRO Struct T n' m') :
+    pro_rewriting_domain p -> pro_rewriting_domain q -> pro_rewriting_domain (p * q);
+  (* pro_rewriting_relation_equiv {n m} :: Equivalence (pro_rewriting_relation n m); *)
+  pro_rewriting_relation_refl {n m} (p : PRO Struct T n m) :
+    pro_rewriting_domain p -> pro_rewriting_relation n m p p;
+  pro_rewriting_relation_symm {n m} :: Symmetric (pro_rewriting_relation n m);
+  pro_rewriting_relation_trans {n m} :: Transitive (pro_rewriting_relation n m);
+  pro_rewriting_relation_graph_syntax_l {n m} (p p' q : PRO Struct T n m) :
+    pro_rewriting_domain p' ->
+    PRO_graph_semantics p ≡ₛ PRO_graph_semantics p' ->
+    pro_rewriting_relation n m p q ->
+    pro_rewriting_relation n m p' q;
+  pro_rewriting_relation_compose {n m o} ::
+    Proper (pro_rewriting_relation n m ==> pro_rewriting_relation m o
+    ==> pro_rewriting_relation n o) Pcompose;
+  pro_rewriting_relation_stack {n m n' m'} ::
+    Proper (pro_rewriting_relation n m ==> pro_rewriting_relation n' m'
+    ==> pro_rewriting_relation (n + n') (m + m')) Pstack;
+}.
+
+Coercion pro_rewriting_relation : LawfulPRORewritingRelation >-> Funclass.
+
+Global Arguments LawfulPRORewritingRelation (_ _) {_ _ _} : assert.
+
+Global Arguments pro_rewriting_relation {_ _ _ _ _} {_} {_ _} _ _ : assert.
+
+
+Lemma pro_rewriting_relation_graph_syntax_r `{StructG : StructGraphable Struct T}
+  `{EqT : Equiv T, EquivT : Equivalence T equiv}
+  (R : LawfulPRORewritingRelation Struct T)
+  {n m} (p q q' : PRO Struct T n m) :
+    pro_rewriting_domain R q' ->
+    R n m p q ->
+    PRO_graph_semantics q ≡ₛ PRO_graph_semantics q' ->
+    R n m p q'.
+Proof.
+  intros Hq' Hqp%symmetry Hqq'.
+  apply (pro_rewriting_relation_graph_syntax_l R q q' p Hq' Hqq') in Hqp.
+  now symmetry.
+Qed.
+
+
+
+
+
+
+
+
+
+
+
+From TensorRocq Require Import ProLike.
+
+Program Definition LawfulProLike_LawfulPRORewritingRelation
+  (R : Type) `{SR : SemiRing R rO rI radd rmul req} (A : Type)
+  `{SA : Summable A, EQA : EqDecision A, WFA : !WFSummable A}
+  (Struct : Mor nat) (T : Type) (D : Mor nat)
+  {ProD : ProLike Struct T D}
+  `{EqT : Equiv T, EquivT : Equivalence T equiv}
+  `{EqStruct : forall n m, Equiv (Struct n m)}
+  `{EquivStruct : forall n m, @Equivalence (Struct n m) equiv}
+  {TensStruct : StrictTensorLike R A Struct}
+  {TensT : TensorLike R A T}
+  {TensD : StrictTensorLike R A D}
+  (LawPro : LawfulProLike R A Struct T D)
+  `{GraphS : StructGraphable Struct T,
+    LawGraphS : !LawfulStructGraphable Struct T}
+  `{StructD : StructableDiagram Struct D,
+    LawStructD : !LawfulStructableDiagram R A Struct D}
+  : LawfulPRORewritingRelation Struct T := {|
+  pro_rewriting_relation n m :=
+    λ p q, exists d1 d2, DiagramDenote d1 p /\ DiagramDenote d2 q /\ d1 ≡ d2;
+  pro_rewriting_domain n m p := is_Some (PRO_to_diagram p);
+|}.
+Next Obligation.
+  intros.
+  cbn; done.
+Qed.
+Next Obligation.
+  intros.
+  cbn; done.
+Qed.
+Next Obligation.
+  cbn.
+  intros.
+  now apply omap2_is_Some.
+Qed.
+Next Obligation.
+  cbn.
+  intros.
+  now apply omap2_is_Some.
+Qed.
+Next Obligation.
+  cbn.
+  intros * ? * ? ? ? ? ?.
+  intros n m p [d Hd].
+  exists d, d.
+  split_and!; [constructor; apply eq_reflexivity, Hd..|].
+  done.
+Qed.
+Next Obligation.
+  cbn.
+  intros * ? * ? ? ? ? ?.
+  unfold Symmetric.
+  naive_solver.
+Qed.
+Next Obligation.
+  cbn.
+  intros * ? * ? ? ? ? ?.
+  intros n m p q r (dp & dq & Hdp & Hdq & Hdpq)
+    (dq' & dr & Hdq' & Hdr & Hdqr).
+  exists dp, dr.
+  split_and!; [done..|].
+  rewrite Hdpq, <- Hdqr.
+  eapply denote_unique; eauto.
+Qed.
+Next Obligation.
+  cbn.
+  intros * ? * ? ? ? ? ?.
+  intros n m p p' q [dp' Hdp'] Hpp' (dp & dq & Hdp & Hdq & Hdpq).
+  exists dp', dq.
+  split_and!; [now constructor; apply eq_reflexivity|done|].
+  rewrite <- Hdpq.
+  destruct Hdp as [Hdp].
+  apply option_relation_Forall2 in Hdp.
+  destruct (PRO_to_diagram p) as [dp''|] eqn:Hdp''; [|done].
+  cbn in Hdp.
+  rewrite <- Hdp.
+  apply (PRO_to_diagram_correct R A) in Hdp', Hdp''.
+  symmetry.
+  apply (Dsemantics_correct R A).
+  rewrite Hdp', Hdp''.
+  rewrite <- 2 (PRO_graph_semantics_correct (LawGraphS:=LawGraphS)).
+  now apply graph_semantics_syntactic_eq.
+Qed.
+Next Obligation.
+  cbn.
+  intros * ? * ? ? ? ? ?.
+  intros n m o p p' (dp & dp' & Hdp & Hdp' & Hdpp') q q' (dq & dq' & Hdq & Hdq' & Hdqq').
+  eexists _, _.
+  split; [apply _|].
+  split; [apply _|].
+  now f_equiv.
+Qed.
+Next Obligation.
+  cbn.
+  intros * ? * ? ? ? ? ?.
+  intros n m n' m' p p' (dp & dp' & Hdp & Hdp' & Hdpp') q q' (dq & dq' & Hdq & Hdq' & Hdqq').
+  eexists _, _.
+  split; [apply _|].
+  split; [apply _|].
+  now f_equiv.
+Qed.
+
+Import PropGraphTerm.
+
+
+
+
+
+
+
+
+
+
+
+
+
+
+
+
+
+
+Definition PRO_monog_context_domainb `{StructGraphable Struct T, Countable T}
+  (R : LawfulPRORewritingRelation Struct T)
+  (graph_to_term : forall n m, CospanHyperGraph T n m -> option (PRO Struct T n m))
+  {i j n m}
+  (ctx : {k & CospanHyperGraph T n (k + i) * CospanHyperGraph T (k + j) m}%type) :
+  bool :=
+  default false (
+    let '(existT k (GC1, GC2)) := ctx in
+    C1 ← graph_to_term _ _ GC1;
+    C2 ← graph_to_term _ _ GC2;
+    _ ← guard (R.(pro_rewriting_domain) C1);
+    _ ← guard (R.(pro_rewriting_domain) C2);
+    Some true).
+
+Lemma PRO_monog_context_domainb_correct `{StructGraphable Struct T, Countable T}
+  (R : LawfulPRORewritingRelation Struct T)
+  (graph_to_term : forall n m, CospanHyperGraph T n m -> option (PRO Struct T n m))
+  (Hgraph_to_term : forall n m cohg p, graph_to_term n m cohg = Some p ->
+    PRO_graph_semantics p ≡ₛ cohg)
+  {i j n m}
+  (ctx : {k & CospanHyperGraph T n (k + i) * CospanHyperGraph T (k + j) m}%type) :
+  PRO_monog_context_domainb R graph_to_term ctx ->
+  forall lhs rhs, R i j lhs rhs ->
+  forall (tl tr : PRO Struct T n m),
+    R.(pro_rewriting_domain) tl ->
+    R.(pro_rewriting_domain) tr ->
+    PRO_graph_semantics tl ≡ₛ make_monog_pushout (PRO_graph_semantics lhs) ctx ->
+    PRO_graph_semantics tr ≡ₛ make_monog_pushout (PRO_graph_semantics rhs) ctx ->
+    R n m tl tr.
+Proof.
+  unfold PRO_monog_context_domainb.
+  destruct ctx as [k [GC1 GC2]].
+  destruct (graph_to_term _ _ GC1) as [C1|] eqn:HC1; [|done].
+  destruct (graph_to_term _ _ GC2) as [C2|] eqn:HC2; [|done].
+  cbn.
+  do 2 case_guard; [|done..].
+  cbn.
+  intros _.
+  intros lhs rhs Hlrhs tl tr HRtl HRtr Htl Htr.
+  eapply pro_rewriting_relation_graph_syntax_l with ((C1 ;; Pid k * lhs) ;; C2)%pro; [done|..].
+  1: {
+    cbn.
+    rewrite Htl.
+    apply compose_graphs_cohg_syntactic_eq, Hgraph_to_term, HC2.
+    apply compose_graphs_cohg_syntactic_eq; [apply Hgraph_to_term, HC1|].
+    done.
+  }
+  eapply pro_rewriting_relation_graph_syntax_r with ((C1 ;; Pid k * rhs) ;; C2)%pro; [done|..].
+  2: {
+    cbn.
+    rewrite Htr.
+    apply compose_graphs_cohg_syntactic_eq, Hgraph_to_term, HC2.
+    apply compose_graphs_cohg_syntactic_eq; [apply Hgraph_to_term, HC1|].
+    done.
+  }
+  f_equiv; [|now apply pro_rewriting_relation_refl].
+  f_equiv; [now apply pro_rewriting_relation_refl|].
+  f_equiv; [|done].
+  apply pro_rewriting_relation_refl.
+  apply R.(pro_rewriting_domain_id).
+Qed.
+
+
+
+Definition PRO_monog_rewrite `{StructGraphable Struct T, Countable T}
+  (R : LawfulPRORewritingRelation Struct T)
+  (graph_to_term : forall n m, CospanHyperGraph T n m -> option (PRO Struct T n m))
+  {i j} (lhs rhs : PRO Struct T i j) {n m} (tgt : PRO Struct T n m)
+  (match_number : nat) :
+  option (PRO Struct T n m) :=
+  let Glhs := PRO_graph_semantics lhs in let Gtgt := PRO_graph_semantics tgt in
+  ctx ← select_monog_context Glhs Gtgt match_number;
+  if negb (default_graph_iso_test Gtgt (make_monog_pushout Glhs ctx)) then None else
+  (* '(existT k (GC1, GC2)) ← select_monog_context Glhs Gtgt match_number; *)
+  if negb (PRO_monog_context_domainb R graph_to_term ctx) then None else
+  let Grhs := PRO_graph_semantics rhs in
+  res ← graph_to_term n m (make_monog_pushout Grhs ctx);
+  _ ← guard (R.(pro_rewriting_domain) res);
+  Some res.
+
+
+Lemma PRO_monog_rewrite_correct `{StructGraphable Struct T, Countable T}
+  (R : LawfulPRORewritingRelation Struct T)
+  (graph_to_term : forall n m, CospanHyperGraph T n m -> option (PRO Struct T n m))
+  (Hgraph_to_term : forall n m cohg p, graph_to_term n m cohg = Some p ->
+    PRO_graph_semantics p ≡ₛ cohg)
+  {i j} (lhs rhs : PRO Struct T i j) {n m} (tgt : PRO Struct T n m)
+  (match_number : nat) :
+  pro_rewriting_domain R tgt ->
+  R i j lhs rhs ->
+  forall res, PRO_monog_rewrite R graph_to_term lhs rhs tgt match_number = Some res ->
+  R n m tgt res.
+Proof.
+  intros Htgt Hlrhs res.
+  unfold PRO_monog_rewrite.
+  set (Glhs := PRO_graph_semantics lhs).
+  set (Grhs := PRO_graph_semantics rhs).
+  set (Gtgt := PRO_graph_semantics tgt).
+  destruct (select_monog_context _ _ _) as [ctx|]; [|done].
+  cbn.
+  destruct (default_graph_iso_test_correct' Gtgt (make_monog_pushout Glhs ctx))
+    as [Hctx|]; [|done].
+  cbn.
+  destruct (PRO_monog_context_domainb _ _ _) as [|] eqn:Hdom; [|done].
+  cbn.
+  specialize (PRO_monog_context_domainb_correct R graph_to_term Hgraph_to_term
+    ctx (Is_true_true_2 _ Hdom)) as Hpush.
+  destruct (graph_to_term _ _ _) as [res'|] eqn:Hres; [|done].
+  cbn.
+  case_guard as Hres'; [|done].
+  cbn.
+  intros [= ->].
+  apply (Hpush lhs rhs Hlrhs).
+  - done.
+  - done.
+  - done.
+  - now apply Hgraph_to_term in Hres.
+Qed.
+
+
+Definition PRO_monog_quote_context_domainb `{StructGraphable Struct T, Countable T',
+  EqT : Equiv T, EquivT : Equivalence T equiv}
+  (R : LawfulPRORewritingRelation Struct T)
+  (graph_to_term : forall n m, CospanHyperGraph T' n m -> option (PRO Struct T' n m))
+  (f : T' -> T)
+  {i j n m}
+  (ctx : {k & CospanHyperGraph T' n (k + i) * CospanHyperGraph T' (k + j) m}%type) :
+  bool :=
+  default false (
+    let '(existT k (GC1, GC2)) := ctx in
+    C1 ← graph_to_term _ _ GC1;
+    C2 ← graph_to_term _ _ GC2;
+    _ ← @guard (R.(pro_rewriting_domain) (PRO_denote f C1)) (R.(pro_rewriting_domain_dec) _);
+    _ ← @guard (R.(pro_rewriting_domain) (PRO_denote f C2)) (R.(pro_rewriting_domain_dec) _);
+    Some true).
+
+Lemma PRO_monog_quote_context_domainb_correct `{FreeStructGraphable Struct,
+  EqStruct : forall n m, Equiv (Struct n m),
+  EquivStruct : forall n m, Equivalence (≡@{Struct n m}),
+  EqT : Equiv T, EquivT : Equivalence T equiv, Countable T'}
+  {StructGProp : forall T (EqT : Equiv T) n m,
+    Proper ((≡@{Struct n m}) ==> cohg_syntactic_eq) (graph_of_struct (T:=T))}
+  (R : LawfulPRORewritingRelation Struct T)
+  (graph_to_term : forall n m, CospanHyperGraph T' n m -> option (PRO Struct T' n m))
+  (Hgraph_to_term : forall n m cohg p, graph_to_term n m cohg = Some p ->
+    PRO_graph_semantics p ≡ₛ cohg)
+  (f : T' -> T) {Hf : Proper (equiv ==> equiv) f}
+  {i j n m}
+  (ctx : {k & CospanHyperGraph T' n (k + i) * CospanHyperGraph T' (k + j) m}%type) :
+  PRO_monog_quote_context_domainb R graph_to_term f ctx ->
+  forall lhs rhs, R i j lhs rhs ->
+  forall Qlhs Qrhs,
+  PRO_quote f Qlhs lhs -> PRO_quote f Qrhs rhs ->
+
+  forall (tl tr : PRO Struct T n m),
+    R.(pro_rewriting_domain) tl ->
+    R.(pro_rewriting_domain) tr ->
+    forall Qtl Qtr,
+    PRO_quote f Qtl tl -> PRO_quote f Qtr tr ->
+    PRO_graph_semantics Qtl ≡ₛ make_monog_pushout (PRO_graph_semantics Qlhs) ctx ->
+    PRO_graph_semantics Qtr ≡ₛ make_monog_pushout (PRO_graph_semantics Qrhs) ctx ->
+    R n m tl tr.
+Proof.
+  unfold PRO_monog_quote_context_domainb.
+  destruct ctx as [k [GC1 GC2]].
+  destruct (graph_to_term _ _ GC1) as [C1|] eqn:HC1; [|done].
+  destruct (graph_to_term _ _ GC2) as [C2|] eqn:HC2; [|done].
+  cbn.
+  do 2 case_guard; [|done..].
+  cbn.
+  intros _.
+  intros lhs rhs Hlrhs Qlhs Qrhs HQlhs HQrhs
+    tl tr HRtl HRtr Qtl Qtr HQtl HQtr Htl Htr.
+  apply (PRO_quote_correct_graph_semantics f) in HQlhs as HQlhs'.
+  apply (PRO_quote_correct_graph_semantics f) in HQrhs as HQrhs'.
+  apply (PRO_quote_correct_graph_semantics f) in HQtl as HQtl'.
+  apply (PRO_quote_correct_graph_semantics f) in HQtr as HQtr'.
+  eapply pro_rewriting_relation_graph_syntax_l with
+    ((PRO_denote f C1 ;; Pid k * lhs) ;; PRO_denote f C2)%pro; [done|..].
+  1: {
+    cbn.
+    rewrite 2 PRO_graph_semantics_denote.
+    rewrite HQlhs'.
+    rewrite <- (graph_apply_hom_id_graph f).
+    rewrite <- graph_apply_hom_stack_graphs.
+    rewrite <- 2 graph_apply_hom_compose_graphs.
+    rewrite HQtl'.
+    f_equiv.
+    rewrite Htl.
+    apply compose_graphs_cohg_syntactic_eq, Hgraph_to_term, HC2.
+    apply compose_graphs_cohg_syntactic_eq; [apply Hgraph_to_term, HC1|].
+    done.
+  }
+  eapply pro_rewriting_relation_graph_syntax_r with
+    ((PRO_denote f C1 ;; Pid k * rhs) ;; PRO_denote f C2)%pro; [done|..].
+  2: {
+    cbn.
+    rewrite 2 PRO_graph_semantics_denote.
+    rewrite HQrhs'.
+    rewrite <- (graph_apply_hom_id_graph f).
+    rewrite <- graph_apply_hom_stack_graphs.
+    rewrite <- 2 graph_apply_hom_compose_graphs.
+    rewrite HQtr'.
+    rewrite Htr.
+    f_equiv.
+    apply compose_graphs_cohg_syntactic_eq, Hgraph_to_term, HC2.
+    apply compose_graphs_cohg_syntactic_eq; [apply Hgraph_to_term, HC1|].
+    done.
+  }
+  f_equiv; [|now apply pro_rewriting_relation_refl].
+  f_equiv; [now apply pro_rewriting_relation_refl|].
+  f_equiv; [|done].
+  apply pro_rewriting_relation_refl.
+  apply R.(pro_rewriting_domain_id).
+Qed.
+
+
+
+Definition PRO_monog_quote_rewrite `{FreeStructGraphable Struct, Countable T',
+  EqT : Equiv T, EquivT : Equivalence T equiv}
+  (R : LawfulPRORewritingRelation Struct T)
+  (graph_to_term : forall n m, CospanHyperGraph T' n m -> option (PRO Struct T' n m))
+  (f : T' -> T)
+  {i j} (Qlhs Qrhs : PRO Struct T' i j) {n m} (Qtgt : PRO Struct T' n m)
+  (match_number : nat) :
+  option (PRO Struct T' n m) :=
+  let Glhs := PRO_graph_semantics Qlhs in let Gtgt := PRO_graph_semantics Qtgt in
+  ctx ← select_monog_context Glhs Gtgt match_number;
+  if negb (default_graph_iso_test Gtgt (make_monog_pushout Glhs ctx)) then None else
+  (* '(existT k (GC1, GC2)) ← select_monog_context Glhs Gtgt match_number; *)
+  if negb (PRO_monog_quote_context_domainb R graph_to_term f ctx) then None else
+  let Grhs := PRO_graph_semantics Qrhs in
+  res ← graph_to_term n m (make_monog_pushout Grhs ctx);
+  (* _ ← guard (R.(pro_rewriting_domain) (PRO_denote f res)); *)
+  Some res.
+
+
+Lemma PRO_monog_quote_rewrite_correct `{FreeStructGraphable Struct,
+  EqStruct : forall n m, Equiv (Struct n m),
+  EquivStruct : forall n m, Equivalence (≡@{Struct n m}),
+  EqT : Equiv T, EquivT : Equivalence T equiv, Countable T'}
+  {StructGProp : forall T (EqT : Equiv T) n m,
+    Proper ((≡@{Struct n m}) ==> cohg_syntactic_eq) (graph_of_struct (T:=T))}
+  (R : LawfulPRORewritingRelation Struct T)
+  (graph_to_term : forall n m, CospanHyperGraph T' n m -> option (PRO Struct T' n m))
+  (Hgraph_to_term : forall n m cohg p, graph_to_term n m cohg = Some p ->
+    PRO_graph_semantics p ≡ₛ cohg)
+  (f : T' -> T) {Hf : Proper (equiv ==> equiv) f}
+  {i j} (lhs rhs : PRO Struct T i j) {n m} (tgt : PRO Struct T n m)
+  (match_number : nat) :
+  pro_rewriting_domain R tgt ->
+  R i j lhs rhs ->
+  forall Qlhs Qrhs Qtgt,
+  PRO_quote f Qlhs lhs ->
+  PRO_quote f Qrhs rhs ->
+  PRO_quote f Qtgt tgt ->
+  forall Qres, PRO_monog_quote_rewrite R graph_to_term f Qlhs Qrhs Qtgt match_number = Some Qres ->
+  forall res, PRO_unquote f Qres res ->
+  bool_decide (R.(pro_rewriting_domain) res) ->
+  R n m tgt res.
+Proof.
+  intros Htgt Hlrhs Qlhs Qrhs Qtgt HQlhs HQrhs HQtgt.
+  unfold PRO_monog_quote_rewrite.
+  set (Glhs := PRO_graph_semantics Qlhs).
+  set (Grhs := PRO_graph_semantics Qrhs).
+  set (Gtgt := PRO_graph_semantics Qtgt).
+  destruct (select_monog_context _ _ _) as [ctx|]; [|done].
+  cbn.
+  destruct (default_graph_iso_test_correct' Gtgt (make_monog_pushout Glhs ctx))
+    as [Hctx|]; [|done].
+  cbn.
+  destruct (PRO_monog_quote_context_domainb _ _ _ _) as [|] eqn:Hdom; [|done].
+  cbn.
+  specialize (PRO_monog_quote_context_domainb_correct R graph_to_term Hgraph_to_term
+    f
+    ctx (Is_true_true_2 _ Hdom)) as Hpush.
+  destruct (graph_to_term _ _ _) as [Qres|] eqn:HQres_eq; [|done].
+  cbn.
+  intros _ [= <-].
+  intros res HQres Hres%bool_decide_spec.
+  eapply (Hpush lhs rhs Hlrhs Qlhs Qrhs HQlhs HQrhs _ _ Htgt Hres Qtgt Qres HQtgt HQres).
+  - done.
+  - apply Hgraph_to_term in HQres_eq.
+    rewrite HQres_eq.
+    apply (PRO_quote_correct_graph_semantics f) in HQrhs as HQrhs'.
+    done.
+Qed.
+
+Lemma LawfulProLike_PRO_monog_quote_rewrite_correct `{Countable T'}
+  (R : Type) `{SR : SemiRing R rO rI radd rmul req} (A : Type)
+  `{SA : Summable A, EQA : EqDecision A, WFA : !WFSummable A}
+  (Struct : Mor nat) (T : Type) (D : Mor nat)
+  {ProD : ProLike Struct T D}
+  `{EqT : Equiv T, EquivT : Equivalence T equiv}
+  `{EqStruct : forall n m, Equiv (Struct n m)}
+  `{EquivStruct : forall n m, @Equivalence (Struct n m) equiv}
+  {TensStruct : StrictTensorLike R A Struct}
+  {TensT : TensorLike R A T}
+  {TensD : StrictTensorLike R A D}
+  (LawPro : LawfulProLike R A Struct T D)
+  `{FreeGraphS : FreeStructGraphable Struct,
+    LawGraphS : !LawfulStructGraphable Struct T}
+  `{StructD : StructableDiagram Struct D,
+    LawStructD : !LawfulStructableDiagram R A Struct D}
+  (RW : LawfulPRORewritingRelation Struct T :=
+    LawfulProLike_LawfulPRORewritingRelation R A Struct T D LawPro)
+
+  {StructGProp : forall T (EqT : Equiv T) n m,
+    Proper ((≡@{Struct n m}) ==> cohg_syntactic_eq) (graph_of_struct (T:=T))}
+  `{StructMon : !SubStruct Monoidal Struct,
+    StructSymm : !SubStruct Symmetry Struct}
+  `{StructClean : CleanableStruct Struct,
+    StructComp : ComposableStruct Struct}
+  (graph_to_term : forall n m, CospanHyperGraph T' n m -> option (PRO Struct T' n m)
+    := fun n m => graph_to_PROP')
+
+  (f : T' -> T) {Hf : Proper (equiv ==> equiv) f}
+  {i j} (dlhs drhs : D i j) {n m} (dtgt : D n m)
+  (match_number : nat) :
+  dlhs ≡ drhs ->
+  forall lhs rhs tgt,
+  DiagramQuote dlhs lhs ->
+  DiagramQuote drhs rhs ->
+  DiagramQuote dtgt tgt ->
+(*
+  pro_rewriting_domain R tgt ->
+  R i j lhs rhs -> *)
+  forall Qlhs Qrhs Qtgt,
+  PRO_quote f Qlhs lhs ->
+  PRO_quote f Qrhs rhs ->
+  PRO_quote f Qtgt tgt ->
+  forall Qres, PRO_monog_quote_rewrite RW graph_to_term f Qlhs Qrhs Qtgt match_number = Some Qres ->
+  forall res, PRO_unquote f Qres res ->
+  forall dres, DiagramDenote dres res ->
+  dtgt ≡ dres.
+Proof.
+  intros Hdlrhs lhs rhs tgt Hlhs Hrhs Htgt.
+  specialize (PRO_monog_quote_rewrite_correct
+    RW graph_to_term (fun n m => graph_to_PROP'_correct) f lhs rhs tgt match_number) as Hrw.
+  tspecialize Hrw. 1:{
+    destruct Htgt as [Htgt].
+    apply (f_equiv is_Some) in Htgt.
+    apply Htgt.
+    done.
+  }
+  tspecialize Hrw by
+    (exists dlhs, drhs; split_and!;
+      [apply DiagramQuote_iff_DiagramDenote..|]; done).
+  intros Qlhs Qrhs Qtgt HQlhs HQrhs HQtgt Qres HQres_eq res HQres dres Hdres.
+  specialize (Hrw Qlhs Qrhs Qtgt HQlhs HQrhs HQtgt Qres HQres_eq res HQres).
+  tspecialize Hrw. 1:{
+    apply bool_decide_spec.
+    destruct Hdres as [Hdres].
+    apply (f_equiv is_Some) in Hdres.
+    now apply Hdres.
+  }
+  destruct Hrw as (dtgt' & dres' & Hdtgt' & Hres' & Hdtgt_res').
+  assert (Hdtgt_tgt' : dtgt ≡ dtgt') by (
+    apply DiagramQuote_iff_DiagramDenote in Htgt;
+    eapply (denote_unique _ _ tgt); eauto).
+  assert (Hdres_res' : dres ≡ dres') by (
+    eapply (denote_unique _ _ res); eauto).
+  rewrite Hdtgt_tgt', Hdres_res'.
+  done.
+Qed.
+
+
+
+
+Definition PRO_context_domainb `{StructGraphable Struct T, Countable T}
+  (R : LawfulPRORewritingRelation Struct T)
+  (graph_to_term : forall n m, CospanHyperGraph T n m -> option (PRO Struct T n m))
+  {i j n m}
+  (ctx : CospanHyperGraph T n ((i + j) + m)) :
+  bool :=
+  default false (
+    Pctx ← graph_to_term _ _ ctx;
+    _ ← guard (R.(pro_rewriting_domain) Pctx);
+    Some true).
+
+Lemma PRO_context_domainb_correct `{Countable T} 
+  `{!SubStruct Autonomy Struct}
+  `{!StructGraphable Struct T}
+  `{!SubStructGraphable Autonomy Struct T}
+  (R : LawfulPRORewritingRelation Struct T)
+  (graph_to_term : forall n m, CospanHyperGraph T n m -> option (PRO Struct T n m))
+  (Hgraph_to_term : forall n m cohg p, graph_to_term n m cohg = Some p ->
+    PRO_graph_semantics p ≡ₛ cohg)
+  {i j n m}
+  (ctx : CospanHyperGraph T n ((i + j) + m)) :
+  PRO_context_domainb R graph_to_term ctx ->
+  forall lhs rhs, R i j lhs rhs ->
+  forall (tl tr : PRO Struct T n m),
+    R.(pro_rewriting_domain) tl ->
+    R.(pro_rewriting_domain) tr ->
+    PRO_graph_semantics tl ≡ₛ make_pushout (PRO_graph_semantics lhs) ctx ->
+    PRO_graph_semantics tr ≡ₛ make_pushout (PRO_graph_semantics rhs) ctx ->
+    R n m tl tr.
+Proof.
+  unfold PRO_context_domainb.
+  destruct (graph_to_term _ _ ctx) as [Pctx|] eqn:HPctx; [|done].
+  cbn.
+  case_guard; [|done].
+  cbn.
+  intros _.
+  intros lhs rhs Hlrhs tl tr HRtl HRtr Htl Htr.
+  eapply pro_rewriting_relation_graph_syntax_l with 
+    (Pctx ;; (lhs * Pid j ;; Pcap j) * Pid m)%pro; [done|..].
+  1: {
+    cbn.
+    rewrite Htl.
+    rewrite graph_of_struct_includeStruct.
+    apply compose_graphs_cohg_syntactic_eq; [apply Hgraph_to_term, HPctx|].
+    done.
+  }
+  eapply pro_rewriting_relation_graph_syntax_r with 
+    (Pctx ;; (rhs * Pid j ;; Pcap j) * Pid m)%pro; [done|..].
+  2: {
+    cbn.
+    rewrite Htr.
+    rewrite graph_of_struct_includeStruct.
+    apply compose_graphs_cohg_syntactic_eq; [apply Hgraph_to_term, HPctx|].
+    done.
+  }
+  f_equiv; [now apply pro_rewriting_relation_refl|].
+  f_equiv; [|apply pro_rewriting_relation_refl, R.(pro_rewriting_domain_id)].
+  f_equiv; [|apply pro_rewriting_relation_refl, R.(pro_rewriting_domain_struct)].
+  f_equiv; [|apply pro_rewriting_relation_refl, R.(pro_rewriting_domain_id)].
+  done.
+Qed.
+
+Definition PRO_gen_rewrite `{StructGraphable Struct T, Countable T}
+  (R : LawfulPRORewritingRelation Struct T)
+  (graph_to_term : forall n m, CospanHyperGraph T n m -> option (PRO Struct T n m))
+  (select_context : forall i j (lhs : CospanHyperGraph T i j)
+    n m (tgt : CospanHyperGraph T n m), nat -> nat -> 
+    option (CospanHyperGraph T n ((i + j) + m)))
+  {i j} (lhs rhs : PRO Struct T i j) {n m} (tgt : PRO Struct T n m)
+  (match_number : nat) (quotient_number : nat) :
+  option (PRO Struct T n m) :=
+  let Glhs := PRO_graph_semantics lhs in let Gtgt := PRO_graph_semantics tgt in
+  ctx ← select_context i j Glhs n m Gtgt match_number quotient_number;
+  if negb (default_graph_iso_test Gtgt (make_pushout Glhs ctx)) then None else
+  (* '(existT k (GC1, GC2)) ← select_monog_context Glhs Gtgt match_number; *)
+  if negb (PRO_context_domainb R graph_to_term ctx) then None else
+  let Grhs := PRO_graph_semantics rhs in
+  res ← graph_to_term n m (make_pushout Grhs ctx);
+  _ ← guard (R.(pro_rewriting_domain) res);
+  Some res.
+
+
+
+
+Definition PRO_bimonog_rewrite `{StructGraphable Struct T, Countable T}
+  (R : LawfulPRORewritingRelation Struct T)
+  (graph_to_term : forall n m, CospanHyperGraph T n m -> option (PRO Struct T n m))
+  {i j} (lhs rhs : PRO Struct T i j) {n m} (tgt : PRO Struct T n m)
+  (match_number quotient_number : nat) :
+  option (PRO Struct T n m) :=
+  PRO_gen_rewrite R graph_to_term (fun i j lhs n m tgt => 
+    select_bimonog_context lhs tgt) lhs rhs tgt match_number quotient_number.
+
+
+Definition PRO_frobenius_rewrite `{StructGraphable Struct T, Countable T}
+  (R : LawfulPRORewritingRelation Struct T)
+  (graph_to_term : forall n m, CospanHyperGraph T n m -> option (PRO Struct T n m))
+  {i j} (lhs rhs : PRO Struct T i j) {n m} (tgt : PRO Struct T n m)
+  (match_number quotient_number : nat) :
+  option (PRO Struct T n m) :=
+  PRO_gen_rewrite R graph_to_term (fun i j lhs n m tgt => 
+    select_frobenius_context lhs tgt) lhs rhs tgt match_number quotient_number.
+
+
+Lemma PRO_gen_rewrite_correct `{Countable T} 
+  `{!SubStruct Autonomy Struct}
+  `{!StructGraphable Struct T}
+  `{!SubStructGraphable Autonomy Struct T}
+  (R : LawfulPRORewritingRelation Struct T)
+  (graph_to_term : forall n m, CospanHyperGraph T n m -> option (PRO Struct T n m))
+  (Hgraph_to_term : forall n m cohg p, graph_to_term n m cohg = Some p ->
+    PRO_graph_semantics p ≡ₛ cohg)
+  (select_context : forall i j (lhs : CospanHyperGraph T i j)
+    n m (tgt : CospanHyperGraph T n m), nat -> nat -> 
+    option (CospanHyperGraph T n ((i + j) + m)))
+  {i j} (lhs rhs : PRO Struct T i j) {n m} (tgt : PRO Struct T n m)
+  (match_number quotient_number : nat) :
+  pro_rewriting_domain R tgt ->
+  R i j lhs rhs ->
+  forall res, PRO_gen_rewrite R graph_to_term select_context 
+    lhs rhs tgt match_number quotient_number = Some res ->
+  R n m tgt res.
+Proof.
+  intros Htgt Hlrhs res.
+  unfold PRO_gen_rewrite.
+  set (Glhs := PRO_graph_semantics lhs).
+  set (Grhs := PRO_graph_semantics rhs).
+  set (Gtgt := PRO_graph_semantics tgt).
+  destruct (select_context _ _ _  _ _ _  _ _) as [ctx|]; [|done].
+  cbn.
+  destruct (default_graph_iso_test_correct' Gtgt (make_pushout Glhs ctx))
+    as [Hctx|]; [|done].
+  cbn.
+  destruct (PRO_context_domainb _ _ _) as [|] eqn:Hdom; [|done].
+  cbn.
+  specialize (PRO_context_domainb_correct R graph_to_term Hgraph_to_term
+    ctx (Is_true_true_2 _ Hdom)) as Hpush.
+  destruct (graph_to_term _ _ _) as [res'|] eqn:Hres; [|done].
+  cbn.
+  case_guard as Hres'; [|done].
+  cbn.
+  intros [= ->].
+  apply (Hpush lhs rhs Hlrhs).
+  - done.
+  - done.
+  - done.
+  - now apply Hgraph_to_term in Hres.
+Qed.
+
+
+Definition PRO_quote_context_domainb `{StructGraphable Struct T, Countable T',
+  EqT : Equiv T, EquivT : Equivalence T equiv}
+  (R : LawfulPRORewritingRelation Struct T)
+  (graph_to_term : forall n m, CospanHyperGraph T' n m -> option (PRO Struct T' n m))
+  (f : T' -> T)
+  {i j n m}
+  (ctx : CospanHyperGraph T' n ((i + j) + m)) :
+  bool :=
+  default false (
+    Pctx ← graph_to_term _ _ ctx;
+    _ ← @guard (R.(pro_rewriting_domain) (PRO_denote f Pctx)) (R.(pro_rewriting_domain_dec) _);
+    Some true).
+
+Lemma PRO_quote_context_domainb_correct `{FreeStructGraphable Struct,
+  EqStruct : forall n m, Equiv (Struct n m),
+  EquivStruct : forall n m, Equivalence (≡@{Struct n m}),
+  EqT : Equiv T, EquivT : Equivalence T equiv, Countable T'}
+  {StructGProp : forall T (EqT : Equiv T) n m,
+    Proper ((≡@{Struct n m}) ==> cohg_syntactic_eq) (graph_of_struct (T:=T))}
+  `{!SubStruct Autonomy Struct, !SubStructGraphable Autonomy Struct T}
+  
+  (R : LawfulPRORewritingRelation Struct T)
+  (graph_to_term : forall n m, CospanHyperGraph T' n m -> option (PRO Struct T' n m))
+  (Hgraph_to_term : forall n m cohg p, graph_to_term n m cohg = Some p ->
+    PRO_graph_semantics p ≡ₛ cohg)
+  (f : T' -> T) {Hf : Proper (equiv ==> equiv) f}
+  {i j n m}
+  (ctx : CospanHyperGraph T' n ((i + j) + m)) :
+  PRO_quote_context_domainb R graph_to_term f ctx ->
+  forall lhs rhs, R i j lhs rhs ->
+  forall Qlhs Qrhs,
+  PRO_quote f Qlhs lhs -> PRO_quote f Qrhs rhs ->
+
+  forall (tl tr : PRO Struct T n m),
+    R.(pro_rewriting_domain) tl ->
+    R.(pro_rewriting_domain) tr ->
+    forall Qtl Qtr,
+    PRO_quote f Qtl tl -> PRO_quote f Qtr tr ->
+    PRO_graph_semantics Qtl ≡ₛ make_pushout (PRO_graph_semantics Qlhs) ctx ->
+    PRO_graph_semantics Qtr ≡ₛ make_pushout (PRO_graph_semantics Qrhs) ctx ->
+    R n m tl tr.
+Proof.
+  unfold PRO_quote_context_domainb.
+  destruct (graph_to_term _ _ ctx) as [Pctx|] eqn:Hctx; [|done].
+  cbn.
+  case_guard; [|done..].
+  cbn.
+  intros _.
+  intros lhs rhs Hlrhs Qlhs Qrhs HQlhs HQrhs
+    tl tr HRtl HRtr Qtl Qtr HQtl HQtr Htl Htr.
+  apply (PRO_quote_correct_graph_semantics f) in HQlhs as HQlhs'.
+  apply (PRO_quote_correct_graph_semantics f) in HQrhs as HQrhs'.
+  apply (PRO_quote_correct_graph_semantics f) in HQtl as HQtl'.
+  apply (PRO_quote_correct_graph_semantics f) in HQtr as HQtr'.
+  eapply pro_rewriting_relation_graph_syntax_l with
+    (PRO_denote f Pctx ;; (lhs * Pid j ;; Pcap j) * Pid m)%pro; [done|..].
+  1: {
+    cbn.
+    rewrite PRO_graph_semantics_denote.
+    rewrite HQlhs'.
+    rewrite graph_of_struct_includeStruct.
+    rewrite <- (graph_apply_hom_id_graph f).
+    rewrite <- (graph_apply_hom_id_graph f (n:=m)).
+    cbn.
+    rewrite <- (graph_apply_hom_cap_graph f).
+    rewrite <- graph_apply_hom_stack_graphs.
+    rewrite <- graph_apply_hom_compose_graphs.
+    rewrite <- graph_apply_hom_stack_graphs.
+    rewrite <- graph_apply_hom_compose_graphs.
+    rewrite HQtl'.
+    f_equiv.
+    cbn.
+    rewrite Htl.
+    unfold make_pushout.
+    f_equiv.
+    apply Hgraph_to_term; done.
+  }
+  eapply pro_rewriting_relation_graph_syntax_r with
+    (PRO_denote f Pctx ;; (rhs * Pid j ;; Pcap j) * Pid m)%pro; [done|..].
+  2: {
+    cbn.
+    rewrite PRO_graph_semantics_denote.
+    rewrite HQrhs'.
+    rewrite graph_of_struct_includeStruct.
+    rewrite <- (graph_apply_hom_id_graph f).
+    rewrite <- (graph_apply_hom_id_graph f (n:=m)).
+    cbn.
+    rewrite <- (graph_apply_hom_cap_graph f).
+    rewrite <- graph_apply_hom_stack_graphs.
+    rewrite <- graph_apply_hom_compose_graphs.
+    rewrite <- graph_apply_hom_stack_graphs.
+    rewrite <- graph_apply_hom_compose_graphs.
+    rewrite HQtr'.
+    f_equiv.
+    cbn.
+    rewrite Htr.
+    unfold make_pushout.
+    f_equiv.
+    apply Hgraph_to_term; done.
+  }
+  f_equiv; [now apply pro_rewriting_relation_refl|].
+  f_equiv; [|apply pro_rewriting_relation_refl, R.(pro_rewriting_domain_id)].
+  f_equiv; [|apply pro_rewriting_relation_refl, R.(pro_rewriting_domain_struct)].
+  f_equiv; [|apply pro_rewriting_relation_refl, R.(pro_rewriting_domain_id)].
+  done.
+Qed.
+
+
+Definition PRO_gen_quote_rewrite `{FreeStructGraphable Struct, Countable T',
+  EqT : Equiv T, EquivT : Equivalence T equiv}
+  (R : LawfulPRORewritingRelation Struct T)
+  (graph_to_term : forall n m, CospanHyperGraph T' n m -> option (PRO Struct T' n m))
+  (select_context : forall i j (lhs : CospanHyperGraph T' i j)
+    n m (tgt : CospanHyperGraph T' n m), nat -> nat -> 
+    option (CospanHyperGraph T' n ((i + j) + m)))
+  (f : T' -> T)
+  {i j} (Qlhs Qrhs : PRO Struct T' i j) {n m} (Qtgt : PRO Struct T' n m)
+  (match_number quotient_number : nat) :
+  option (PRO Struct T' n m) :=
+  let Glhs := PRO_graph_semantics Qlhs in let Gtgt := PRO_graph_semantics Qtgt in
+  ctx ← select_context i j Glhs n m Gtgt match_number quotient_number;
+  if negb (default_graph_iso_test Gtgt (make_pushout Glhs ctx)) then None else
+  (* '(existT k (GC1, GC2)) ← select_monog_context Glhs Gtgt match_number; *)
+  if negb (PRO_quote_context_domainb R graph_to_term f ctx) then None else
+  let Grhs := PRO_graph_semantics Qrhs in
+  res ← graph_to_term n m (make_pushout Grhs ctx);
+  (* _ ← guard (R.(pro_rewriting_domain) res); *)
+  Some res.
+
+
+Lemma PRO_gen_quote_rewrite_correct `{FreeStructGraphable Struct,
+  EqStruct : forall n m, Equiv (Struct n m),
+  EquivStruct : forall n m, Equivalence (≡@{Struct n m}),
+  EqT : Equiv T, EquivT : Equivalence T equiv, Countable T'}
+  {StructGProp : forall T (EqT : Equiv T) n m,
+    Proper ((≡@{Struct n m}) ==> cohg_syntactic_eq) (graph_of_struct (T:=T))}
+  `{!SubStruct Autonomy Struct, !SubStructGraphable Autonomy Struct T}
+
+  (R : LawfulPRORewritingRelation Struct T)
+  (graph_to_term : forall n m, CospanHyperGraph T' n m -> option (PRO Struct T' n m))
+  (Hgraph_to_term : forall n m cohg p, graph_to_term n m cohg = Some p ->
+    PRO_graph_semantics p ≡ₛ cohg)
+  select_context
+  (f : T' -> T) {Hf : Proper (equiv ==> equiv) f}
+  {i j} (lhs rhs : PRO Struct T i j) {n m} (tgt : PRO Struct T n m)
+  (match_number quotient_number : nat) :
+  pro_rewriting_domain R tgt ->
+  R i j lhs rhs ->
+  forall Qlhs Qrhs Qtgt,
+  PRO_quote f Qlhs lhs ->
+  PRO_quote f Qrhs rhs ->
+  PRO_quote f Qtgt tgt ->
+  forall Qres, PRO_gen_quote_rewrite R graph_to_term select_context
+    f Qlhs Qrhs Qtgt match_number quotient_number = Some Qres ->
+  forall res, PRO_unquote f Qres res ->
+  bool_decide (R.(pro_rewriting_domain) res) ->
+  R n m tgt res.
+Proof.
+  intros Htgt Hlrhs Qlhs Qrhs Qtgt HQlhs HQrhs HQtgt.
+  unfold PRO_gen_quote_rewrite.
+  set (Glhs := PRO_graph_semantics Qlhs).
+  set (Grhs := PRO_graph_semantics Qrhs).
+  set (Gtgt := PRO_graph_semantics Qtgt).
+  
+  destruct (select_context _ _ _  _ _ _  _ _) as [ctx|]; [|done].
+  cbn.
+  destruct (default_graph_iso_test_correct' Gtgt (make_pushout Glhs ctx))
+    as [Hctx|]; [|done].
+  cbn.
+  destruct (PRO_quote_context_domainb _ _ _ _) as [|] eqn:Hdom; [|done].
+  cbn.
+  specialize (PRO_quote_context_domainb_correct R graph_to_term Hgraph_to_term
+    f ctx (Is_true_true_2 _ Hdom)) as Hpush.
+  destruct (graph_to_term _ _ _) as [Qres|] eqn:HQres_eq; [|done].
+  cbn.
+  intros _ [= <-].
+  intros res HQres Hres%bool_decide_spec.
+  eapply (Hpush lhs rhs Hlrhs Qlhs Qrhs HQlhs HQrhs _ _ Htgt Hres Qtgt Qres HQtgt HQres).
+  - done.
+  - apply Hgraph_to_term in HQres_eq.
+    rewrite HQres_eq.
+    apply (PRO_quote_correct_graph_semantics f) in HQrhs as HQrhs'.
+    done.
+Qed.
+
+(* FIXME: Move *)
+#[export] Instance substruct_symmetricg_of_monoidal_symmetry 
+  `{!SubStruct Monoidal Struct, !SubStruct Symmetry Struct} : 
+  SubStruct SymmetricG Struct := fun n m s =>
+  match s with
+  | inl s | inr s => includeStruct s
+  end.
+
+#[export] Instance substruct_autonomous_of_symmetricg_autonomy 
+  `{!SubStruct SymmetricG Struct, !SubStruct Autonomy Struct} : 
+  SubStruct Autonomous Struct := fun n m s =>
+  match s with
+  | inl s | inr s => includeStruct s
+  end.
+
+#[export] Instance substruct_frobenius_of_autonomous_frobenial
+  `{!SubStruct Autonomous Struct, !SubStruct Frobenial Struct} : 
+  SubStruct Frobenius Struct := fun n m s =>
+  match s with
+  | inl s | inr s => includeStruct s
+  end.
+
+
+
+Lemma LawfulProLike_PRO_bimonog_quote_rewrite_correct `{Countable T'}
+  (R : Type) `{SR : SemiRing R rO rI radd rmul req} (A : Type)
+  `{SA : Summable A, EQA : EqDecision A, WFA : !WFSummable A}
+  (Struct : Mor nat) (T : Type) (D : Mor nat)
+  {ProD : ProLike Struct T D}
+  `{EqT : Equiv T, EquivT : Equivalence T equiv}
+  `{EqStruct : forall n m, Equiv (Struct n m)}
+  `{EquivStruct : forall n m, @Equivalence (Struct n m) equiv}
+  {TensStruct : StrictTensorLike R A Struct}
+  {TensT : TensorLike R A T}
+  {TensD : StrictTensorLike R A D}
+  (LawPro : LawfulProLike R A Struct T D)
+  `{FreeGraphS : FreeStructGraphable Struct,
+    LawGraphS : !LawfulStructGraphable Struct T}
+  `{StructD : StructableDiagram Struct D,
+    LawStructD : !LawfulStructableDiagram R A Struct D}
+  (RW : LawfulPRORewritingRelation Struct T :=
+    LawfulProLike_LawfulPRORewritingRelation R A Struct T D LawPro)
+
+  {StructGProp : forall T (EqT : Equiv T) n m,
+    Proper ((≡@{Struct n m}) ==> cohg_syntactic_eq) (graph_of_struct (T:=T))}
+  `{StructMono : !SubStruct Monoidal Struct,
+    StructSymm : !SubStruct Symmetry Struct,
+    StructAuto : !SubStruct Autonomy Struct,
+    SubStructG : !SubStructGraphable Autonomy Struct T}
+  `{StructClean : CleanableStruct Struct,
+    StructComp : ComposableStruct Struct}
+  (graph_to_term : forall n m, CospanHyperGraph T' n m -> option (PRO Struct T' n m)
+    := fun n m => graph_to_APROP')
+  (select_context := fun i j lhs n m tgt => 
+    select_bimonog_context lhs tgt)
+
+  (f : T' -> T) {Hf : Proper (equiv ==> equiv) f}
+  {i j} (dlhs drhs : D i j) {n m} (dtgt : D n m)
+  (match_number quotient_number : nat) :
+  dlhs ≡ drhs ->
+  forall lhs rhs tgt,
+  DiagramQuote dlhs lhs ->
+  DiagramQuote drhs rhs ->
+  DiagramQuote dtgt tgt ->
+(*
+  pro_rewriting_domain R tgt ->
+  R i j lhs rhs -> *)
+  forall Qlhs Qrhs Qtgt,
+  PRO_quote f Qlhs lhs ->
+  PRO_quote f Qrhs rhs ->
+  PRO_quote f Qtgt tgt ->
+  forall Qres, PRO_gen_quote_rewrite RW graph_to_term select_context f
+    Qlhs Qrhs Qtgt match_number quotient_number = Some Qres ->
+  forall res, PRO_unquote f Qres res ->
+  forall dres, DiagramDenote dres res ->
+  dtgt ≡ dres.
+Proof.
+  intros Hdlrhs lhs rhs tgt Hlhs Hrhs Htgt.
+  specialize (PRO_gen_quote_rewrite_correct
+    RW graph_to_term (fun n m => graph_to_APROP'_correct) select_context 
+    f lhs rhs tgt match_number quotient_number) as Hrw.
+  tspecialize Hrw. 1:{
+    destruct Htgt as [Htgt].
+    apply (f_equiv is_Some) in Htgt.
+    apply Htgt.
+    done.
+  }
+  tspecialize Hrw by
+    (exists dlhs, drhs; split_and!;
+      [apply DiagramQuote_iff_DiagramDenote..|]; done).
+  intros Qlhs Qrhs Qtgt HQlhs HQrhs HQtgt Qres HQres_eq res HQres dres Hdres.
+  specialize (Hrw Qlhs Qrhs Qtgt HQlhs HQrhs HQtgt Qres HQres_eq res HQres).
+  tspecialize Hrw. 1:{
+    apply bool_decide_spec.
+    destruct Hdres as [Hdres].
+    apply (f_equiv is_Some) in Hdres.
+    now apply Hdres.
+  }
+  destruct Hrw as (dtgt' & dres' & Hdtgt' & Hres' & Hdtgt_res').
+  assert (Hdtgt_tgt' : dtgt ≡ dtgt') by (
+    apply DiagramQuote_iff_DiagramDenote in Htgt;
+    eapply (denote_unique _ _ tgt); eauto).
+  assert (Hdres_res' : dres ≡ dres') by (
+    eapply (denote_unique _ _ res); eauto).
+  rewrite Hdtgt_tgt', Hdres_res'.
+  done.
+Qed.
+
+Lemma LawfulProLike_PRO_frobenius_quote_rewrite_correct `{Countable T'}
+  (R : Type) `{SR : SemiRing R rO rI radd rmul req} (A : Type)
+  `{SA : Summable A, EQA : EqDecision A, WFA : !WFSummable A}
+  (Struct : Mor nat) (T : Type) (D : Mor nat)
+  {ProD : ProLike Struct T D}
+  `{EqT : Equiv T, EquivT : Equivalence T equiv}
+  `{EqStruct : forall n m, Equiv (Struct n m)}
+  `{EquivStruct : forall n m, @Equivalence (Struct n m) equiv}
+  {TensStruct : StrictTensorLike R A Struct}
+  {TensT : TensorLike R A T}
+  {TensD : StrictTensorLike R A D}
+  (LawPro : LawfulProLike R A Struct T D)
+  `{FreeGraphS : FreeStructGraphable Struct,
+    LawGraphS : !LawfulStructGraphable Struct T}
+  `{StructD : StructableDiagram Struct D,
+    LawStructD : !LawfulStructableDiagram R A Struct D}
+  (RW : LawfulPRORewritingRelation Struct T :=
+    LawfulProLike_LawfulPRORewritingRelation R A Struct T D LawPro)
+
+  {StructGProp : forall T (EqT : Equiv T) n m,
+    Proper ((≡@{Struct n m}) ==> cohg_syntactic_eq) (graph_of_struct (T:=T))}
+  `{StructMono : !SubStruct Monoidal Struct,
+    StructSymm : !SubStruct Symmetry Struct,
+    StructAuto : !SubStruct Autonomy Struct,
+    StructFrob : !SubStruct Frobenial Struct,
+    SubStructG : !SubStructGraphable Autonomy Struct T}
+  `{StructClean : CleanableStruct Struct,
+    StructComp : ComposableStruct Struct}
+  (graph_to_term : forall n m, CospanHyperGraph T' n m -> option (PRO Struct T' n m)
+    := fun n m => graph_to_FPROP')
+  (select_context := fun i j lhs n m tgt => 
+    select_frobenius_context lhs tgt)
+
+  (f : T' -> T) {Hf : Proper (equiv ==> equiv) f}
+  {i j} (dlhs drhs : D i j) {n m} (dtgt : D n m)
+  (match_number quotient_number : nat) :
+  dlhs ≡ drhs ->
+  forall lhs rhs tgt,
+  DiagramQuote dlhs lhs ->
+  DiagramQuote drhs rhs ->
+  DiagramQuote dtgt tgt ->
+(*
+  pro_rewriting_domain R tgt ->
+  R i j lhs rhs -> *)
+  forall Qlhs Qrhs Qtgt,
+  PRO_quote f Qlhs lhs ->
+  PRO_quote f Qrhs rhs ->
+  PRO_quote f Qtgt tgt ->
+  forall Qres, PRO_gen_quote_rewrite RW graph_to_term select_context f
+    Qlhs Qrhs Qtgt match_number quotient_number = Some Qres ->
+  forall res, PRO_unquote f Qres res ->
+  forall dres, DiagramDenote dres res ->
+  dtgt ≡ dres.
+Proof.
+  intros Hdlrhs lhs rhs tgt Hlhs Hrhs Htgt.
+  specialize (PRO_gen_quote_rewrite_correct
+    RW graph_to_term (fun n m => graph_to_FPROP'_correct) select_context 
+    f lhs rhs tgt match_number quotient_number) as Hrw.
+  tspecialize Hrw. 1:{
+    destruct Htgt as [Htgt].
+    apply (f_equiv is_Some) in Htgt.
+    apply Htgt.
+    done.
+  }
+  tspecialize Hrw by
+    (exists dlhs, drhs; split_and!;
+      [apply DiagramQuote_iff_DiagramDenote..|]; done).
+  intros Qlhs Qrhs Qtgt HQlhs HQrhs HQtgt Qres HQres_eq res HQres dres Hdres.
+  specialize (Hrw Qlhs Qrhs Qtgt HQlhs HQrhs HQtgt Qres HQres_eq res HQres).
+  tspecialize Hrw. 1:{
+    apply bool_decide_spec.
+    destruct Hdres as [Hdres].
+    apply (f_equiv is_Some) in Hdres.
+    now apply Hdres.
+  }
+  destruct Hrw as (dtgt' & dres' & Hdtgt' & Hres' & Hdtgt_res').
+  assert (Hdtgt_tgt' : dtgt ≡ dtgt') by (
+    apply DiagramQuote_iff_DiagramDenote in Htgt;
+    eapply (denote_unique _ _ tgt); eauto).
+  assert (Hdres_res' : dres ≡ dres') by (
+    eapply (denote_unique _ _ res); eauto).
+  rewrite Hdtgt_tgt', Hdres_res'.
+  done.
+Qed.
+
+
+
+
+
+
+(*
+
+
+
+
+
+Record PROPushout {Struct T} := mk_PROPushout {
+  pro_pushout_context (i j n m : nat) :> Type;
+  pro_mk_pushout {i j n m}
+    (ctx : pro_pushout_context i j n m)
+    (lhs : PRO Struct T i j) : PRO Struct T n m;
+}.
+
+Global Arguments PROPushout _ _ : clear implicits, assert.
+
+Record PROMatchingEngine {Struct T} {P : PROPushout Struct T} := mk_PROMatchingEngine {
+  pro_match_selector :> Type;
+  pro_match {i j} (subp : PRO Struct T i j) {n m} (tgt : PRO Struct T n m)
+    (s : pro_match_selector) : option (P i j n m);
+}.
+
+Global Arguments PROMatchingEngine {_ _} (_) : assert.
+
+Record PRORewritingEngine {Struct T} {P : PROPushout Struct T}
+  {M : PROMatchingEngine P} := mk_PRORewritingEngine {
+  pro_rewrite {i j} (lhs rhs : PRO Struct T i j) {n m} (tgt : PRO Struct T n m)
+    (match_number : M) : option (PRO Struct T n m);
+}.
+
+Global Arguments PRORewritingEngine {_ _} (_ _) : assert.
+
+Class LawfulPRORewritingEngine {Struct T} {StructG : StructGraphable Struct T}
+  `{EqT : Equiv T, EquivT : Equivalence T equiv}
+  (P : PROPushout Struct T) (M : PROMatchingEngine P)
+  (RW : PRORewritingEngine P M) (R : LawfulPRORewritingRelation Struct T) := {
+  pro_rewrite_spec {i j} (lhs rhs : PRO Struct T i j) {n m} (tgt : PRO Struct T n m)
+    (s : M) res : RW.(pro_rewrite) lhs rhs tgt s = Some res ->
+      R i j lhs rhs ->
+      R n m tgt res
+}.
+
+
+
+Definition PRORW_of_test_match {Struct T}
+  {P : PROPushout Struct T} (M : PROMatchingEngine P)
+  ()
+
+
+
+
+
+
+
+
+
+
+
+
+
+
+
+
+
+
+
+
+
+
+
+Class LawfulPROPushout {Struct T} {StructG : StructGraphable Struct T}
+  `{EqT : Equiv T, EquivT : Equivalence T equiv}
+  (P : PROPushout Struct T) (R : LawfulPRORewritingRelation Struct T) := {
+  pro_mk_pushout_proper i j n m ctx ::
+    Proper (R i j ==> R n m) (P.(pro_mk_pushout) ctx)
+}.
+
+Class LawfulPROMatchingEngine {Struct T} {StructG : StructGraphable Struct T}
+  `{EqT : Equiv T, EquivT : Equivalence T equiv}
+  (P : PROPushout Struct T)
+  (M : PROMatchingEngine P) (R : LawfulPRORewritingRelation Struct T) := {
+  lawful_pro_match_pushout :: LawfulPROPushout P R;
+  pro_match_correct {i j} (subp : PRO Struct T i j) {n m} (tgt : PRO Struct T n m)
+    (s : M) ctx : M.(pro_match) subp tgt s = Some ctx ->
+      R n m tgt (P.(pro_mk_pushout) ctx subp);
+  pro_match_dom {i j} (subp : PRO Struct T i j) {n m} (tgt : PRO Struct T n m)
+    (s : M) ctx : M.(pro_match) subp tgt s = Some ctx ->
+      forall subp', R.(pro_rewriting_domain) subp' ->
+      R.(pro_rewriting_domain) (P.(pro_mk_pushout) ctx subp');
+}.
+
+Class LawfulPRORewritingEngine {Struct T} {StructG : StructGraphable Struct T}
+  `{EqT : Equiv T, EquivT : Equivalence T equiv}
+  (P : PROPushout Struct T) (M : PROMatchingEngine P)
+  (RW : PRORewritingEngine P M) (R : LawfulPRORewritingRelation Struct T) := {
+  lawful_pro_rewrite_match :: LawfulPROMatchingEngine P M R;
+  pro_rewrite_spec {i j} (lhs rhs : PRO Struct T i j) {n m} (tgt : PRO Struct T n m)
+    (s : M) res : RW.(pro_rewrite) lhs rhs tgt s = Some res ->
+      exists ctx, M.(pro_match) lhs tgt s = Some ctx
+        /\ R n m res (P.(pro_mk_pushout) ctx rhs);
+}.
+
+Lemma pro_rewrite_correct {Struct T} {StructG : StructGraphable Struct T}
+  `{EqT : Equiv T, EquivT : Equivalence T equiv}
+  (P : PROPushout Struct T) (M : PROMatchingEngine P)
+  (RW : PRORewritingEngine P M) (R : LawfulPRORewritingRelation Struct T)
+  {LawRW : LawfulPRORewritingEngine P M RW R}
+  {i j} (lhs rhs : PRO Struct T i j) {n m} (tgt : PRO Struct T n m)
+    (s : M) res :
+    R i j lhs rhs ->
+    RW.(pro_rewrite) lhs rhs tgt s = Some res ->
+    R n m tgt res.
+Proof.
+  intros Hlhs_rhs Hrew.
+  apply pro_rewrite_spec in Hrew as Hctx.
+  destruct Hctx as (ctx & Hmatch & Hres).
+  rewrite Hres.
+  rewrite <- Hlhs_rhs.
+  now apply pro_match_correct in Hmatch.
+Qed.
+
+
+
+
+
+Definition nth_frobenius_context
+  `{Countable T}
+  {i j} (lhs : CospanHyperGraph T i j)
+  {n m} (cohg : CospanHyperGraph T n m)
+  (match_number : nat) :
+  option (CospanHyperGraph T n (i + j + m)) :=
+  ctx ← all_frobenius_contexts lhs cohg !! match_number;
+  if opt_weak_graph_iso_partial_test (make_pushout lhs ctx) cohg
+    then Some ctx
+  else None.
+
+
+
+
+
+
+Lemma DiagramQuote_to_DiagramDenote_correct_rew {Struct T D} `{ProD : ProLike Struct T D}
+  `{EqT : Equiv T, EquivT : Equivalence T equiv}
+  `{EqStruct : forall n m, Equiv (Struct n m)}
+  `{EquivStruct : forall n m, @Equivalence (Struct n m) equiv}
+  {TensStruct : StrictTensorLike R A Struct}
+  {TensT : TensorLike R A T}
+  {TensD : StrictTensorLike R A D}
+  (LawProD : LawfulProLike Struct T D)
+  {i j} (lhs rhs : PRO Struct T i j) (dlhs drhs : D i j)
+  {n m} (tgt res : PRO Struct T n m) (dtgt : D n m) :
+  DiagramQuote dlhs lhs -> DiagramDenote drhs rhs ->
+
+  DiagramQuote dtgt tgt ->
+  forall res,
+
+  DiagramDenote d' p' ->
+  PRO_semantics p ≡ PRO_semantics p' ->
+  d ≡ d'.
+Proof.
+  rewrite <- DiagramQuote_iff_DiagramDenote.
+  apply DiagramQuote_correct.
+Qed. *)
